Auto/Tactic.lean
@@ -199,20 +199,22 @@ def runAuto (instrstx : TSyntax ``autoinstr) (lemmas : Array Lemma) : TacticM Re
     let afterReify (ufacts : Array UMonoFact) : LamReif.ReifM Expr := (do
       let exportFacts ← LamReif.reifFacts ufacts
       let exportFacts ← exportFacts.mapM (fun t => LamReif.skolemizeMostIntoForall (.validEVar0 [] t))
+      let exportFacts ← exportFacts.mapM LamReif.validOfExtensionalize
+      let exportFacts ← exportFacts.mapM LamReif.validOfBetaReduce
       let exportFacts ← exportFacts.mapM LamReif.validOfRevertAll
       -- ! smt
-      try
-        let lamVarTy := (← LamReif.getVarVal).map Prod.snd
-        let lamEVarTy ← LamReif.getLamEVarTy
-        let exportLamTerms ← exportFacts.mapM (fun re => do
-          match re.getValid? with
-          | .some ([], t) => return t | _ => throwError "runAuto :: Unexpected error")
-        let commands ← (lamFOL2SMT lamVarTy lamEVarTy exportLamTerms).run'
-        for cmd in commands do
-          trace[auto.smt.printCommands] "Command: {cmd}"
-        Solver.SMT.querySolver commands
-      catch e =>
-        trace[auto.smt.result] "SMT invocation failed with {e.toMessageData}"
+      -- try
+      --   let lamVarTy := (← LamReif.getVarVal).map Prod.snd
+      --   let lamEVarTy ← LamReif.getLamEVarTy
+      --   let exportLamTerms ← exportFacts.mapM (fun re => do
+      --     match re.getValid? with
+      --     | .some ([], t) => return t | _ => throwError "runAuto :: Unexpected error")
+      --   let commands ← (lamFOL2SMT lamVarTy lamEVarTy exportLamTerms).run'
+      --   for cmd in commands do
+      --     trace[auto.smt.printCommands] "Command: {cmd}"
+      --   Solver.SMT.querySolver commands
+      -- catch e =>
+      --   trace[auto.smt.result] "SMT invocation failed with {e.toMessageData}"
       -- reconstruction
       let (proof, proofLamTerm, usedEtoms, unsatCore) ← Lam2D.callDuper exportFacts
       trace[auto.printProof] "Duper found proof of {← Meta.inferType proof}"
