TODO.md
@@ -1,1 +1,2 @@
 * HOL to FOL. Do this in the verified checker. Introduce new term atoms into varVal to represent instances of higher-order functions.
+* When we matched against ``Eq`` in monomorphization, we found that some type arguments of other constants got unified with ``Prop``, which created a bunch of junk lemma. Find out whether something similar happened in Duper.
